Smallgroups/UsefulTheorems/Order48.lean
@@ -26,4 +26,5 @@ import Smallgroups.UsefulTheorems.Order48.FourSylowThreeRO
 import Smallgroups.UsefulTheorems.Order48.FourSylowThreeActionOrbits
 import Smallgroups.UsefulTheorems.Order48.FourSylowThreeActionClassifiers
 import Smallgroups.UsefulTheorems.Order48.FourSylowThreeG0
+import Smallgroups.UsefulTheorems.Order48.FourSylowThreeG7
 import Smallgroups.UsefulTheorems.Order48.Classification
